ulib/experimental/Steel.PCM.Heap.fsti
@@ -395,6 +395,19 @@ val sel (#a:Type u#h) (#pcm:pcm a) (r:ref a pcm) (m:hheap (ptr r)) : a
 val sel_lemma (#a:_) (#pcm:_) (r:ref a pcm) (m:hheap (ptr r))
   : Lemma (interp (pts_to r (sel r m)) m)
 
+let witnessed_ref (#a:Type u#a)
+                  (#pcm:pcm a)
+                  (r:ref a pcm)
+                  (fact:a -> prop)
+                  (h:heap)
+  = interp (ptr r) h /\
+    fact (sel r h)
+
+val witnessed_ref_stability (#a:Type) (#pcm:pcm a) (r:ref a pcm) (fact:a -> prop)
+  : Lemma
+    (requires FStar.Preorder.stable fact (Steel.PCM.Preorder.preorder_of_pcm pcm))
+    (ensures FStar.Preorder.stable (witnessed_ref r fact) heap_evolves)
+
 (**
   The action variant of [sel], returning the "true" value inside the heap. This "true" value
   can be different of the [pts_to] value you assumed at the beginning, because of the PCM structure
